IMP-_To_SAS+/IMP-_To_IMP--/Binary_Arithmetic.thy
@@ -1,0 +1,105 @@
+\<^marker>\<open>creator Florian Keßler\<close>
+
+section "Binary Arithmetic"
+                                                    
+theory Binary_Arithmetic 
+  imports Main "../IMP_Minus_Minus_Small_StepT"
+begin 
+
+fun nth_bit_nat:: "nat \<Rightarrow> nat \<Rightarrow> nat" where
+"nth_bit_nat x 0 = x mod 2" |
+"nth_bit_nat x (Suc n) = nth_bit_nat (x div 2) n"
+
+definition nth_bit:: "nat \<Rightarrow> nat \<Rightarrow> bit" where
+"nth_bit x n = nat_to_bit (nth_bit_nat x n)" 
+
+lemma nth_bit_of_zero[simp]: "nth_bit 0 n = Zero" 
+  by (induction n) (auto simp: nth_bit_def)
+
+fun nth_carry:: "nat \<Rightarrow> nat \<Rightarrow> nat \<Rightarrow> bit" where
+"nth_carry 0 a b = (if (nth_bit a 0 = One \<and> nth_bit b 0 = One) then One else Zero)" | 
+"nth_carry (Suc n) a b = (if (nth_bit a (Suc n) = One \<and> nth_bit b (Suc n) = One) 
+  \<or> ((nth_bit a (Suc n) = One \<or> nth_bit b (Suc n) = One) \<and> nth_carry n a b = One) 
+  then One else Zero)"
+
+lemma first_bit_of_add: "nth_bit (a + b) 0 
+  = (if nth_bit a 0 = One then if nth_bit b 0 = One then Zero else One 
+     else if nth_bit b 0 = One then One else Zero)" 
+  sorry
+
+lemma nth_bit_of_add: "nth_bit (a + b) (Suc n) = (let u = nth_bit a (Suc n); 
+  v = nth_bit b (Suc n); w = nth_carry n a b in 
+  (if u = One then 
+    if v = One then
+     if w = One then One else Zero
+    else
+     if w = One then Zero else One
+   else
+    if v = One then
+     if w = One then Zero else One
+    else
+     if w = One then One else Zero))"
+  sorry
+
+lemma no_overflow_condition: "a + b < 2^n \<Longrightarrow> nth_carry (n - 1) a b = Zero" 
+  sorry
+
+lemma has_bit_one_then_greater_zero: "nth_bit a j = One \<Longrightarrow> 0 < a" 
+  sorry
+
+lemma greater_zero_then_has_bit_one: "x > 0 \<Longrightarrow> x < 2 ^ n \<Longrightarrow> \<exists>b \<in> {0..<n}. nth_bit x b = One" 
+  sorry
+
+fun nth_carry_sub:: "nat \<Rightarrow> nat \<Rightarrow> nat \<Rightarrow> bit" where
+"nth_carry_sub 0 a b = (if (nth_bit a 0 = Zero \<and> nth_bit b 0 = One) then One else Zero)" | 
+"nth_carry_sub (Suc n) a b = 
+  (if (nth_bit a (Suc n) = Zero \<and> ( nth_bit b (Suc n) = One \<or> nth_carry_sub n a b = One))
+    \<or> (nth_bit a (Suc n) = One \<and> (nth_bit b (Suc n)) = One \<and> nth_carry_sub n a b = One) then One
+  else Zero)"
+
+lemma first_bit_of_sub_n_no_underflow: "a \<ge> b \<Longrightarrow> nth_bit (a - b) 0 = (if nth_bit a 0 = One then
+  (if nth_bit b 0 = One then Zero else One)
+  else (if nth_bit b 0 = One then One else Zero))" 
+  apply(auto simp: nth_bit_def nat_to_bit_eq_One_iff nat_to_bit_eq_Zero_iff)
+  by presburger+
+
+lemma nth_bit_of_sub_n_no_underflow: "a \<ge> b \<Longrightarrow> 
+  nth_bit (a - b) (Suc n) = (let an = nth_bit a (Suc n); bn = nth_bit b (Suc n);
+  c = nth_carry_sub n a b in (if (bn = Zero \<and> c = Zero) \<or> (bn = One \<and> c = One) then an 
+    else (if (bn = One \<or> c = One) \<and> an = Zero then One else Zero)))" 
+  sorry
+
+lemma nth_bit_of_sub_n_underflow: "a < b \<Longrightarrow> 
+  nth_bit (a - b) (Suc n) = Zero" 
+  by simp
+
+lemma nth_carry_sub_underflow: "a < b \<Longrightarrow> a < 2 ^ n \<Longrightarrow> b < 2 ^ n 
+  \<Longrightarrow> nth_carry_sub (n - 1) (2^n + a) b = One" 
+  sorry         
+
+lemma nth_carry_sub_no_underflow: "a \<ge> b \<Longrightarrow> a < 2 ^ n \<Longrightarrow> b < 2 ^ n 
+  \<Longrightarrow> nth_carry_sub (n - 1) a b = Zero" 
+  by (smt bit_neq_zero_iff le_add_diff_inverse no_overflow_condition nth_bit_of_add 
+      nth_bit_of_sub_n_no_underflow)
+
+lemma nth_bit_add_out_of_range: "a < 2 ^ n \<Longrightarrow> j < n \<Longrightarrow> nth_bit (2 ^ n + a) j = nth_bit a j" 
+  sorry
+
+fun bit_list_to_nat:: "bit list \<Rightarrow> nat" where
+"bit_list_to_nat [] = 0" |
+"bit_list_to_nat (x # xs) = (case x of Zero \<Rightarrow> 2 * bit_list_to_nat xs |
+  One \<Rightarrow> 1 + 2 * bit_list_to_nat xs)" 
+
+lemma nth_bit_of_bit_list_to_nat[simp]: "nth_bit (bit_list_to_nat l) k 
+  = (if k < length l then l ! k else Zero)" 
+  sorry
+
+lemma bit_list_to_nat_geq_two_to_the_k_then: "bit_list_to_nat l \<ge> 2 ^ k
+  \<Longrightarrow> (\<exists>i. k \<le> i \<and> i < length l \<and> l ! i = One)" 
+  sorry
+
+lemma bit_list_to_nat_eq_nat_iff: "bit_list_to_nat l = y \<longleftrightarrow> (y < 2 ^ length l \<and>
+  (\<forall>i < length l. l ! i = nth_bit y i))"
+  sorry
+
+end
